Trying something else with lists

src/Assembly.v
@@ -1,90 +1,63 @@
-Require Import Vector.
-Import Vector.VectorNotations.
+Require Import List.
+Import List.ListNotations.
 Require Import Program.Equality.
 Require Import Common.
 Module Assembly.
 
 Inductive instr : Type :=
-  | Load : instr
-  | Store : instr
+  | Load : nat -> instr
+  | Store : nat -> instr
+  | AddPtr : nat -> instr
+  | SubPtr : nat -> instr
   | Add : nat -> instr
   | Sub : nat -> instr
   | Jump : nat -> instr
   | Skip : instr
-  | Swap : instr
-  | Zero : instr
   | Halt : instr
   | UJUMP : instr (* unlinked *)
   | URET : instr (* unlinked *).
 
-Definition program (n : nat) := t instr n. 
-Record state {n m : nat} : Type := mkState
+Definition program := list instr.
+Record state: Type := mkState
 { 
-  prog : @program n;
-  mem : t nat m;
-  pc : Fin.t n;
-  ac : Fin.t m;
-  b : Fin.t m;
+  prog : program;
+  mem : list nat;
+  pc : nat;
+  ac : nat;
 }.
 
-Definition read_instr' {n} (prog : @program n) (pc : Fin.t n) : instr :=
-  prog[@pc].
+Definition read_instr (p : state) (i : instr) :=
+  Common.lookup (prog p) (pc p) i.
 
-Inductive read_instr {n m} (p : state) (i : instr) : Prop :=
-  | ri : read_instr' p.(prog n m) p.(pc) = i -> read_instr p i.
-
-Definition read_mem' {m} (mem : t nat m) (ptr : Fin.t m) : nat := mem[@ptr].
-
-Inductive read_mem {n m} (p : state) (e : nat) : Prop  :=
-  | mi : read_mem' p.(mem n m) p.(ac) = e -> read_mem p e.
-
-Inductive mem_diff {m} (m1 : t nat m) (m2 : t nat m) (x : Fin.t m) : Prop :=
-  | md : (forall i, i <> x -> m2[@i] = m1[@i]) -> mem_diff m1 m2 x. 
-
-
-Fixpoint weaken_fin_t {n : nat} (f : Fin.t n) : Fin.t (S n) :=
-  match f in Fin.t n return Fin.t (S n) with
-  | Fin.F1 => Fin.F1
-  | Fin.FS f' => Fin.FS (weaken_fin_t f')
-  end.
+(*list_eq_except {A} (m1 : list A) (m2 : list A) (indexes : list nat)*)
 
 (* Small-step operational semantics for our target language.*)
 
-Inductive semantics {n m} (p : state) (p' : state) : Prop :=
-  | load : read_instr p (Load) ->  Common.to_nat p.(pc n m) + 1 = Common.to_nat p'.(pc)->
-             p.(prog) = p'.(prog) -> p.(mem) = p'.(mem) -> p.(b) = p'.(b) ->
-             Common.to_nat p'.(ac) = (read_mem' p.(mem) p.(b)) -> semantics p p'
-  | store: read_instr p (Store) -> Common.to_nat p.(pc) + 1 = Common.to_nat p'.(pc) ->
-           p.(prog) = p'.(prog) -> p.(ac) = p'.(ac) ->
-           Common.to_nat p.(ac) = read_mem' p'.(mem) p.(ac) -> p.(b) = p'.(b) ->
-           mem_diff p.(mem) p'.(mem) p.(b) -> semantics p p'
-  | add : forall n', read_instr p (Add n') -> Common.to_nat p.(pc) + 1 =
-              Common.to_nat p'.(pc) -> p.(prog) = p'.(prog) -> p.(mem) = p'.(mem) ->
-              p.(b) = p'.(b) -> Common.to_nat p'.(ac) = Common.to_nat (p.(ac)) + n' ->
-              semantics p p'
-  | sub : forall n', read_instr p (Sub n') -> Common.to_nat p.(pc) + 1 = 
-              Common.to_nat p'.(pc) -> p.(prog) = p'.(prog) -> p.(mem) = p'.(mem) ->
-              p.(b) = p'.(b) -> Common.to_nat p'.(ac) = (Common.to_nat p.(ac)) - n' ->
-              semantics p p'
-  | jump : forall n', read_instr p (Jump n') -> p.(prog) = p'.(prog) ->
-               p.(ac) = p'.(ac) -> p.(mem) = p'.(mem) -> Common.to_nat (p'.(pc)) =
-               n' -> p.(b) = p'.(b) -> semantics p p'
-  | skipz: read_instr p (Skip) -> p.(prog) = p'.(prog) ->
-               p.(mem) = p'.(mem) -> p.(ac) = p'.(ac) -> p.(b) = p'.(b) ->
-               read_mem p 0 -> Common.to_nat (p'.(pc)) = Common.to_nat (p.(pc)) + 2 ->
-               semantics p p'
-  | skipnz: read_instr p (Skip) -> p.(prog) = p'.(prog) ->
-                p.(mem) = p'.(mem) -> p.(ac) = p'.(ac) -> p.(b) = p'.(b) ->
-                ~ (read_mem p 0) -> Common.to_nat p'.(pc) = (Common.to_nat p.(pc)) + 1 ->
-                semantics p p'
-  | swap : read_instr p (Swap) -> p.(prog) =
-           p'.(prog) -> p.(mem) = p'.(mem) ->
-           p.(ac) = p'.(b) -> p.(b) = p'.(ac) -> Common.to_nat p'.(pc) =
-           (Common.to_nat p.(pc)) + 1 ->
-           semantics p p'
-  | zero : read_instr p (Zero) -> p.(prog) =
-           p'.(prog) -> p.(mem) = p'.(mem) ->
-           p'.(b) = p.(b) -> 0 = Common.to_nat p'.(ac) -> Common.to_nat p'.(pc) =
-           (Common.to_nat p.(pc)) + 1 ->
-           semantics p p'.
+Inductive semantics (p p' : state) : Prop :=
+  | load :forall addr, read_instr p (Load addr) ->
+          pc p + 1 = pc p' -> prog p = prog p' -> mem p = mem p' ->
+          Common.lookup (mem p) addr (ac p') -> semantics p p'
+  | store:forall addr, read_instr p (Store addr) ->
+          pc p + 1 = pc p' -> prog p = prog p' -> ac p = ac p' ->
+          Common.list_eq_except (mem p) (mem p') [addr] ->
+          Common.lookup (mem p) addr (ac p) -> semantics p p'
+  | add_ptr : forall addr, read_instr p (AddPtr addr) ->
+          pc p + 1 = pc p' -> prog p = prog p' -> mem p = mem p' ->
+          Common.lookup (mem p) addr (ac p' - ac p) -> semantics p p'
+  | sub_ptr : forall addr, read_instr p (SubPtr addr) ->
+          pc p + 1 = pc p' -> prog p = prog p' -> mem p = mem p' ->
+          Common.lookup (mem p) addr (ac p - ac p') -> semantics p p'
+  | add : forall imm, read_instr p (Add imm) ->
+          pc p + 1 = pc p' -> prog p = prog p' -> mem p = mem p' ->
+          ac p' = ac p + imm -> semantics p p'
+  | sub : forall imm, read_instr p (Sub imm) ->
+          pc p + 1 = pc p' -> prog p = prog p' -> mem p = mem p' ->
+          ac p' = ac p - imm -> semantics p p'
+  | jump: forall addr, read_instr p (Jump addr) ->
+          prog p = prog p' -> mem p = mem p' -> ac p = ac p' ->
+          pc p' = addr -> semantics p p'
+  | skipz: read_instr p Skip -> prog p = prog p' -> mem p = mem p' ->
+           ac p = ac p' -> ac p' = 0 -> pc p' = pc p + 2 -> semantics p p'
+  | skipnz:read_instr p Skip -> prog p = prog p' -> mem p = mem p' ->
+           ac p = ac p' -> ac p' <> 0 -> pc p' = pc p + 1 -> semantics p p'.
 End Assembly.
