src/Compiler.v
@@ -1,198 +1,123 @@
 Require Import Common.
 Require Import Language.
 Require Import Assembly.
-From Hammer Require Import Hammer.
-From Hammer Require Import Tactics.
-Require Import Vector.
-Import Vector.VectorNotations.
-Require Import Program.Equality.
-Require Import PeanoNat.
-Require Import Lia.
-Import Nat.
-Require Import Coq.Vectors.VectorEq.
-Require Coq.Program.Wf.
+
+Require Import List.
+Import List.ListNotations.
 
 Module Compiler.
 
-Definition lenvec {A n} (v : Vector.t A n) : nat := n.
-Fixpoint matched' {n} (p : Language.program n) (c : nat) : bool :=
-  match c with
-  | 0 => false
-  | _ => match p with
-    | [] => c =? 1
-    | Language.Jump :: l => matched' l (c+1)
-    | Language.Ret  :: l => matched' l (c-1)
-    | _ :: l => matched' l c
-    end
-  end.
-
-
-Inductive matched {n} (p : Language.program n) : Prop :=
-  | match_r : matched' p 1 = true -> matched p.
-Fixpoint comp_len {n} (p : Language.program n) : nat :=
-  match p with
-  | Vector.nil _ => 0
-  | Language.PtrInc :: xs => 1 + comp_len xs
-  | Language.PtrDec :: xs => 1 + comp_len xs
-  | Language.Inc :: xs => 6 + comp_len xs
-  | Language.Dec :: xs => 6 + comp_len xs
-  | Language.Jump :: xs => 2 + comp_len xs
-  | Language.Ret :: xs => 2 + comp_len xs
-  | Language.Halt :: xs => 1 + comp_len xs
-  end.
-
-Fixpoint compile'' {n} (p : Language.program n) :
-                          (Assembly.program (comp_len p)) :=
+Fixpoint compile'' (p : Language.program) : Assembly.program :=
   match p with
   | [] => []
-  | Language.PtrInc :: h => (Assembly.Add 1) :: compile'' h
-  | Language.PtrDec :: h => (Assembly.Sub 1) :: compile'' h
-  | Language.Inc :: h =>  Assembly.Swap   ::
-                          Assembly.Load   ::
-                          Assembly.Add 1  ::
-                          Assembly.Store  ::
-                          Assembly.Zero   ::
-                          Assembly.Swap   :: compile'' h
-  | Language.Dec :: h =>  Assembly.Swap   ::
-                          Assembly.Load   ::
-                          Assembly.Sub 1  ::
-                          Assembly.Store  ::
-                          Assembly.Zero   ::
-                          Assembly.Swap   :: compile'' h
-
-  | Language.Jump :: h => Assembly.Skip   ::
-                          Assembly.UJUMP :: compile'' h
-  | Language.Ret :: h =>  Assembly.Skip   ::
-                          Assembly.URET :: compile'' h
+  | Language.PtrInc :: h => Assembly.Add 1 :: compile'' h
+  | Language.PtrDec :: h => Assembly.Sub 1 :: compile'' h
+  | Language.Inc :: h =>  Assembly.AddPtr 1 :: compile'' h
+  | Language.Dec :: h =>  Assembly.SubPtr 1 :: compile'' h
+  | Language.Jump :: h => Assembly.Skip   :: Assembly.UJUMP :: compile'' h
+  | Language.Ret :: h =>  Assembly.Skip   :: Assembly.URET :: compile'' h
   | Language.Halt :: h => Assembly.Halt   :: compile'' h
   end.
 
-Definition compile_first {n : nat} (i : Language.instr) : Assembly.instr :=
-  match i with
+Definition comp_first (x : Language.instr) : Assembly.instr :=
+  match x with
   | Language.PtrInc => Assembly.Add 1
   | Language.PtrDec => Assembly.Sub 1
-  | Language.Inc => Assembly.Swap
-  | Language.Dec => Assembly.Swap
+  | Language.Inc => Assembly.AddPtr 1
+  | Language.Dec => Assembly.SubPtr 1
   | Language.Jump => Assembly.Skip
-  | Language.Ret => Assembly.Skip
+  | Language.Ret =>  Assembly.Skip
   | Language.Halt => Assembly.Halt
   end.
 
-Fixpoint compile_index {n} (p : Language.program n) (x : Fin.t n) 
-                           : Fin.t (comp_len p).
-Proof.
-  destruct x eqn:H1; rewrite (eta p).
-  - destruct hd; apply Fin.F1.
-  - destruct hd.
-    + do 1 apply Fin.FS. apply compile_index. exact t0.
-    + do 1 apply Fin.FS. apply compile_index. exact t0.
-    + do 6 apply Fin.FS. apply compile_index. exact t0.
-    + do 6 apply Fin.FS. apply compile_index. exact t0.
-    + do 2 apply Fin.FS. apply compile_index. exact t0.
-    + do 2 apply Fin.FS. apply compile_index. exact t0.
-    + do 1 apply Fin.FS. apply compile_index. exact t0.
-Defined.
+Fixpoint compile_index (p : Language.program) (x : nat) : nat :=
+  match x with
+  | 0 => 0
+  | _ => match p with
+         | [] => 0
+         | Language.Jump :: h => 2 + compile_index h (x-1)
+         | Language.Ret :: h => 2 + compile_index h (x-1)
+         | _ :: h => 1 + compile_index h (x-1)
+         end
+  end.
 
-Fixpoint nb_jump {n} (p : Assembly.program n) : nat :=
+
+Fixpoint nb_jump (p : Assembly.program) : nat :=
   match p with
   | [] => 0
   | Assembly.UJUMP :: t => 1 + nb_jump t
   | _ :: t => nb_jump t
   end.
 
-Fixpoint nb_ret {n} (p : Assembly.program n) : nat :=
+Fixpoint nb_ret (p : Assembly.program) : nat :=
   match p with
   | [] => 0
   | Assembly.URET :: t => 1 + nb_ret t
   | _ :: t => nb_ret t
   end.
 
-Fixpoint j_indexes {n} (p : Assembly.program n) 
-                       : (Vector.t (Fin.t n) (nb_jump p)) :=
+Fixpoint j_indexes (p : Assembly.program) : list nat :=
   match p with
   | [] => []
-  | Assembly.UJUMP :: t => Fin.F1 :: map Fin.FS (j_indexes t)
-  | _ :: t => map Fin.FS (j_indexes t)
+  | Assembly.UJUMP :: t => 0 :: map S (j_indexes t)
+  | _ :: t => map S (j_indexes t)
   end.
 
-Fixpoint r_indexes {n} (p : Assembly.program n) 
-                       : (Vector.t (Fin.t n) (nb_ret p)) :=
+Fixpoint r_indexes (p : Assembly.program) : list nat :=
   match p with
   | [] => []
-  | Assembly.URET :: t => Fin.F1 :: map Fin.FS (r_indexes t)
-  | _ :: t => map Fin.FS (r_indexes t)
+  | Assembly.URET :: t => 0 :: map S (r_indexes t)
+  | _ :: t => map S (r_indexes t)
   end.
 
-  
+(*
 
-Fixpoint link_jump' {n ln ln'} (p : Assembly.program n) 
-                          (jumps : Vector.t (Fin.t n) ln)
-                          (rets : Vector.t (Fin.t n) ln') :
-                          Assembly.program n :=
+Put a at the p{^ th} place of v
+Fixpoint replace {A n} (v : t A n) (p: Fin.t n) (a : A) {struct p}: t A n :=
+*)
+
+Fixpoint replace (v : list Assembly.instr) (p : nat) (a : Assembly.instr) : list Assembly.instr :=
+  match v with
+  | [] => v
+  | h :: l => match p with
+              | 0 => a :: l
+              | S n => h :: replace l n a
+              end
+  end.
+
+Fixpoint link_jump' (p : Assembly.program) (jumps rets : list nat) :
+                    Assembly.program :=
   match jumps with
   | [] => p
   | a :: jumps' => match rets with
                   | [] => p
-                  | r :: rets' => link_jump' 
-                                  (replace p a (Assembly.Jump 
-                                  (Common.to_nat r)))
-                                  jumps' rets'
+                  | r :: rets' => link_jump' (replace p a (Assembly.Jump r)) jumps' rets'
                   end
   end.
 
-
-Definition link_jump {n} (p : Assembly.program n) : (Assembly.program n) :=
-  link_jump' p (j_indexes p) (r_indexes p).
-
-Fixpoint nb_ljump {n} (p : Assembly.program n) : nat :=
-  match p with
-  | [] => 0
-  | Assembly.Jump _ :: t => 1 + nb_ljump t
-  | _ :: t => nb_ljump t
-  end.
-
-
-Fixpoint lj_indexes {n} (p : Assembly.program n) 
-                        : (Vector.t (Fin.t n) (nb_ljump p)) :=
-  match p with
-  | [] => []
-  | Assembly.Jump _ :: t => Fin.F1 :: map Fin.FS (lj_indexes t)
-  | _ :: t => map Fin.FS (lj_indexes t)
-  end.
-
-
-Definition make_f1 (x : nat) (H : x <> 0) : Fin.t x.
-Proof.
-  destruct x eqn:H1.
-  - auto with *.
-  - exact Fin.F1.
-Defined.
-
-Fixpoint weaken_fin_t {n : nat} (f : Fin.t n) : Fin.t (S n) :=
-  match f in Fin.t n return Fin.t (S n) with
-  | Fin.F1 => Fin.F1
-  | Fin.FS f' => Fin.FS (weaken_fin_t f')
-  end.
-
-Fixpoint make_indexes (n : nat) : Vector.t (Fin.t n) n :=
-  match n with
-  | 0 => []
-  | S i => Fin.F1 :: map Fin.FS (make_indexes i)
-  end.
-
-Fixpoint link_ret' {n ln ln'} (p : Assembly.program n) 
-                          (jumps : Vector.t (Fin.t n) ln) 
-                          (rets : Vector.t (Fin.t n) ln') :
-                          Assembly.program n :=
+Fixpoint link_ret' (p : Assembly.program) (jumps rets : list nat) : Assembly.program :=
   match rets with
   | [] => p
   | a :: rets' => match jumps with
                   | [] => p
-                  | r :: jumps' => link_ret' (replace p a 
-                                   (Assembly.Jump (Common.to_nat r)))
-                                   jumps' rets'
+                  | r :: jumps' => link_ret' (replace p a (Assembly.Jump r)) jumps' rets'
                   end
   end.
+
+
+Definition link_jump (p : Assembly.program) : (Assembly.program) :=
+  link_jump' p (j_indexes p) (r_indexes p).
+
+
+Fixpoint lj_indexes (p : Assembly.program) : list nat :=
+  match p with
+  | [] => []
+  | Assembly.Jump _ :: t => 0 :: map S (lj_indexes t)
+  | _ :: t => map S (lj_indexes t)
+  end.
+
+Definition link_ret (p : Assembly.program) : (Assembly.program) :=
+  (link_ret' p (lj_indexes p) (r_indexes p)).
 
 Definition inc_jump (i : Assembly.instr) : Assembly.instr :=
   match i with
@@ -200,58 +125,22 @@ Definition inc_jump (i : Assembly.instr) : Assembly.instr :=
   | a => a
   end.
 
-Definition link_ret {n} (p : Assembly.program n) : (Assembly.program n) :=
-  (link_ret' p (lj_indexes p) (r_indexes p)).
-
-Definition link {n} (l : Assembly.program n) : (Assembly.program n) :=
+Definition link (l : Assembly.program) : (Assembly.program) :=
   map (inc_jump) (link_ret (link_jump l)).
 
-Definition make_vector (A : Type) (x : A) (n : nat) : Vector.t A n.
-Proof.
-  induction n.
-  - apply Vector.nil.
-  - apply Vector.cons.
-    + exact x.
-    + exact IHn.
-Defined.
+Definition compile' (p : Language.state) : Assembly.state :=
+  Assembly.mkState (link (compile'' (Language.prog p)))
+                   (Language.mem p)
+                   (compile_index (Language.prog p) (Language.pc p))
+                   (Language.ptr p).
 
-Lemma lm1 {n m} : forall p, n <> 0 -> comp_len (@Language.prog n m p) <> 0.
-Proof.
-  intros.
-  destruct p.
-  cbn.
-  destruct prog.
-  inversion pc.
-  unfold not. intros.
-  destruct h; inversion H0.
-Qed.
+Inductive compile (p : Language.state) (q : Assembly.state) : Prop :=
+  | comp : q = compile' p -> compile p q.
 
-Definition compile' {n m}
-  (p : Language.state (n := n)) (HA: n <> 0) (HA2 : m <> 0) : 
-  (Assembly.state (n := comp_len p.(Language.prog)) (m := m)) :=
-  let newlen := comp_len p.(Language.prog) in
-  let newpc := compile_index p.(Language.prog) p.(Language.pc) in
-  let f1_index := make_f1 (comp_len p.(Language.prog)) (lm1 p HA) in
-  let f1_mem := make_f1 m HA2 in
-  @Assembly.mkState newlen m (compile'' p.(Language.prog)) p.(Language.mem)
-   newpc p.(Language.ptr) f1_mem.
-
-Definition compile_link {n m} (p : Language.state (n := n)) (HA : n <> 0)
-                              (HA2 : m <> 0) : 
-  (Assembly.state (n := comp_len p.(Language.prog)) (m := m)) :=
-  let cpl := compile' p HA HA2 in
-  Assembly.mkState (comp_len (Language.prog p)) m (link cpl.(Assembly.prog))
-                   cpl.(Assembly.mem)
-  cpl.(Assembly.pc) cpl.(Assembly.ac) cpl.(Assembly.b).
-
-Inductive compile {n m}
-  (p : Language.state (n := n))
-  (q : Assembly.state (n := comp_len p.(Language.prog)) (m := m)) : Prop :=
-  | comp_r : forall H H1, matched (p.(Language.prog)) -> q 
-             = compile_link p H H1 -> compile p q.
 End Compiler.
-
+(*
 Require Import ExtrOcamlBasic.
 Require Import ExtrOcamlNatInt.
 Extraction Language OCaml.
-Recursive Extraction Compiler.compile_link.
+Recursive Extraction Compiler.compile'.
+*)
