src/prototype/Example.v
@@ -1,107 +1,76 @@
-Require Import Vector.
-Import Vector.VectorNotations.
-Require Import Program.Equality.
-
-Inductive instr1 : Type :=
-  | Load : instr1
-  | Halt : instr1.
-
-Inductive instr2 {n} : Type :=
-  | Load' : instr2
-  | Halt' : Fin.t n -> instr2.
-
-Definition make_f1 (x : nat) (H : x <> 0) : Fin.t x.
-Proof.
-  destruct x eqn:H1.
-  - auto with *.
-  - exact Fin.F1.
-Defined.
-
-Definition comp_instr {n : nat} (HA : n <> 0) x :=
-  match x with
-  | Load => Load'
-  | Halt => Halt' (make_f1 n HA)
-  end.
-
-Fixpoint comp_len {n} (p : t instr1 n) : nat :=
-  match p with
-  | Vector.nil _ => 0
-  | Halt :: xs => 1 + comp_len xs
-  | Load :: xs => 2 + comp_len xs
-  end.
-
-Fixpoint compile' {n n'} (HA : n' <> 0) (p : t instr1 n) : t (@instr2 n') (comp_len p).
-Proof.
-  destruct p.
-  - exact [].
-  - destruct h.
-    + cbn.
-      exact ((Load' :: Load' :: (compile' n n' HA p))).
-    + cbn.
-      exact ((Halt' (make_f1 n' HA)) :: (compile' n n' HA p)).
-Defined.
-
-Fixpoint to_nat {n} (x : Fin.t n) : nat.
-Proof.
-  destruct x eqn:H.
-  - exact 0.
-  - apply plus.
-    + exact 1.
-    + apply to_nat with (n := n).
-      exact t.
-Defined.
-
-Fixpoint weaken_fin_t {n : nat} (f : Fin.t n) : Fin.t (S n) :=
-  match f in Fin.t n return Fin.t (S n) with
-  | Fin.F1 => Fin.F1
-  | Fin.FS f' => Fin.FS (weaken_fin_t f')
-  end.
-Require Import Coq.Program.Wf.
-From Hammer Require Import Tactics.
+Require Import List.
+Require Import Nat.
 Require Import Lia.
-Program Fixpoint fin_t_fact {n} (i : Fin.t n) {measure (to_nat i)} : nat :=
-  match i with
-  | Fin.F1 => 1
-  | Fin.FS t => (to_nat i) * (fin_t_fact (weaken_fin_t t))
+Import ListNotations.
+
+From Hammer Require Import Tactics.
+
+Inductive lookup {A : Type} : list A -> nat -> A -> Prop :=
+  | lu1 : forall x xs, lookup (x :: xs) 0 x
+  | lu2 : forall x xs i y, lookup xs i y -> lookup (x :: xs) (S i) y.
+Inductive instr1 : Type := | Load : instr1 | Halt : instr1.
+Inductive instr2 : Type := | Load' : instr2 | Halt' : instr2.
+Fixpoint compile (p : list instr1) : list instr2 :=
+  match p with
+  | [] => []
+  | Load :: h => Load'::Load'::compile h
+  | Halt :: h => Halt'::compile h
   end.
-Next Obligation.
-  dependent destruction t.
-  - ssimpl.
-  - ssimpl.
-    assert (to_nat (weaken_fin_t t) = to_nat t).
-    + dependent induction t. ssimpl.
-      ssimpl.
-    + rewrite H. lia.
-Qed.
-Check (nat, bool).
-
-Fixpoint make_indexes (n : nat) : Vector.t (Fin.t n) n :=
-  match n with
-  | 0 => []
-  | S i => Fin.F1 :: map Fin.FS (make_indexes i)
+Definition comp_first (i : instr1) : instr2 := 
+  match i with | Halt => Halt' | Load => Load' end.
+Fixpoint compile_index (p : list instr1) (x : nat) : nat :=
+  match x with
+  | 0 => 0
+  | _ => match p with
+         | [] => 0
+         | Load :: h => 2 + compile_index h (x-1)
+         | Halt :: h => 1 + compile_index h (x-1)
+         end
   end.
 
-Compute (make_indexes 8).
-
-Lemma lm1 : forall n p, n <> 0 -> @comp_len n p <> 0.
+Lemma lm6 : forall a p, compile (a :: p) = [] -> False.
 Proof.
-  intros. destruct p. auto with *. destruct h; cbn; auto with *.
+  intros.
+  induction p;
+  destruct a; simpl;
+  discriminate.
 Qed.
-Definition compile {n : nat} (p : t instr1 n) (HA : n <> 0) : t (@instr2 (comp_len p)) (comp_len p) :=
-  @compile' n (comp_len p) (lm1 n p HA) p.
 
-Fixpoint compile_index {n} (p : t instr1 n) (x : Fin.t n) : Fin.t (comp_len p).
+Lemma trv : forall n, n - 0 = n.
+Proof. lia. Qed.
+
+Theorem th :
+  forall p q i x, compile p = q -> lookup p x i ->
+  lookup q (compile_index p x) (comp_first i).
 Proof.
-  destruct x eqn:H1; rewrite (eta p); destruct hd eqn:H2.
-  - apply Fin.F1.
-  - apply Fin.F1.
-  - do 2 apply Fin.FS. apply compile_index. exact t.
-  - do 1 apply Fin.FS, compile_index. exact t.
-Defined.
+  induction p; destruct q; destruct i; intros; try inversion H.
+  - inversion H0.
+  - inversion H0.
+  - exfalso.
+    apply lm6 with (a := a) (p := p).
+    assumption.
+  - exfalso.
+    apply lm6 with (a := a) (p := p).
+    assumption.
+  - ssimpl; apply lu2.
+    rewrite trv.
+    inversion H. apply lu2. apply lu1.
+    apply lu2. apply lu2. assumption.
+  - ssimpl; apply lu2.
+    rewrite trv.
+    apply IHp.
+    reflexivity.
+    assumption.
+Qed.
 
-Theorem th : forall {n} (x : Fin.t n) (p : Vector.t instr1 n) (HA : n <> 0),
-  @comp_instr (comp_len p) (lm1 n p HA) p[@x] = (@compile n p HA)[@compile_index p x].
-Admitted.
-
-
-
+Theorem comp_instr : forall prog pc i, lookup prog pc i ->
+                     lookup (compile prog) (compile_index prog pc) (comp_first i).
+Proof.
+  intros.
+  assert (forall p q i x, compile p = q -> lookup p x i ->
+          lookup q (compile_index p x) (comp_first i)).
+  apply th.
+  apply H0.
+  reflexivity.
+  assumption.
+Qed.
