first_attempt/Assembly.v
@@ -1,0 +1,90 @@
+Require Import Vector.
+Import Vector.VectorNotations.
+Require Import Program.Equality.
+Require Import Common.
+Module Assembly.
+
+Inductive instr : Type :=
+  | Load : instr
+  | Store : instr
+  | Add : nat -> instr
+  | Sub : nat -> instr
+  | Jump : nat -> instr
+  | Skip : instr
+  | Swap : instr
+  | Zero : instr
+  | Halt : instr
+  | UJUMP : instr (* unlinked *)
+  | URET : instr (* unlinked *).
+
+Definition program (n : nat) := t instr n. 
+Record state {n m : nat} : Type := mkState
+{ 
+  prog : @program n;
+  mem : t nat m;
+  pc : Fin.t n;
+  ac : Fin.t m;
+  b : Fin.t m;
+}.
+
+Definition read_instr' {n} (prog : @program n) (pc : Fin.t n) : instr :=
+  prog[@pc].
+
+Inductive read_instr {n m} (p : state) (i : instr) : Prop :=
+  | ri : read_instr' p.(prog n m) p.(pc) = i -> read_instr p i.
+
+Definition read_mem' {m} (mem : t nat m) (ptr : Fin.t m) : nat := mem[@ptr].
+
+Inductive read_mem {n m} (p : state) (e : nat) : Prop  :=
+  | mi : read_mem' p.(mem n m) p.(ac) = e -> read_mem p e.
+
+Inductive mem_diff {m} (m1 : t nat m) (m2 : t nat m) (x : Fin.t m) : Prop :=
+  | md : (forall i, i <> x -> m2[@i] = m1[@i]) -> mem_diff m1 m2 x. 
+
+
+Fixpoint weaken_fin_t {n : nat} (f : Fin.t n) : Fin.t (S n) :=
+  match f in Fin.t n return Fin.t (S n) with
+  | Fin.F1 => Fin.F1
+  | Fin.FS f' => Fin.FS (weaken_fin_t f')
+  end.
+
+(* Small-step operational semantics for our target language.*)
+
+Inductive semantics {n m} (p : state) (p' : state) : Prop :=
+  | load : read_instr p (Load) ->  Common.to_nat p.(pc n m) + 1 = Common.to_nat p'.(pc)->
+             p.(prog) = p'.(prog) -> p.(mem) = p'.(mem) -> p.(b) = p'.(b) ->
+             Common.to_nat p'.(ac) = (read_mem' p.(mem) p.(b)) -> semantics p p'
+  | store: read_instr p (Store) -> Common.to_nat p.(pc) + 1 = Common.to_nat p'.(pc) ->
+           p.(prog) = p'.(prog) -> p.(ac) = p'.(ac) ->
+           Common.to_nat p.(ac) = read_mem' p'.(mem) p.(ac) -> p.(b) = p'.(b) ->
+           mem_diff p.(mem) p'.(mem) p.(b) -> semantics p p'
+  | add : forall n', read_instr p (Add n') -> Common.to_nat p.(pc) + 1 =
+              Common.to_nat p'.(pc) -> p.(prog) = p'.(prog) -> p.(mem) = p'.(mem) ->
+              p.(b) = p'.(b) -> Common.to_nat p'.(ac) = Common.to_nat (p.(ac)) + n' ->
+              semantics p p'
+  | sub : forall n', read_instr p (Sub n') -> Common.to_nat p.(pc) + 1 = 
+              Common.to_nat p'.(pc) -> p.(prog) = p'.(prog) -> p.(mem) = p'.(mem) ->
+              p.(b) = p'.(b) -> Common.to_nat p'.(ac) = (Common.to_nat p.(ac)) - n' ->
+              semantics p p'
+  | jump : forall n', read_instr p (Jump n') -> p.(prog) = p'.(prog) ->
+               p.(ac) = p'.(ac) -> p.(mem) = p'.(mem) -> Common.to_nat (p'.(pc)) =
+               n' -> p.(b) = p'.(b) -> semantics p p'
+  | skipz: read_instr p (Skip) -> p.(prog) = p'.(prog) ->
+               p.(mem) = p'.(mem) -> p.(ac) = p'.(ac) -> p.(b) = p'.(b) ->
+               read_mem p 0 -> Common.to_nat (p'.(pc)) = Common.to_nat (p.(pc)) + 2 ->
+               semantics p p'
+  | skipnz: read_instr p (Skip) -> p.(prog) = p'.(prog) ->
+                p.(mem) = p'.(mem) -> p.(ac) = p'.(ac) -> p.(b) = p'.(b) ->
+                ~ (read_mem p 0) -> Common.to_nat p'.(pc) = (Common.to_nat p.(pc)) + 1 ->
+                semantics p p'
+  | swap : read_instr p (Swap) -> p.(prog) =
+           p'.(prog) -> p.(mem) = p'.(mem) ->
+           p.(ac) = p'.(b) -> p.(b) = p'.(ac) -> Common.to_nat p'.(pc) =
+           (Common.to_nat p.(pc)) + 1 ->
+           semantics p p'
+  | zero : read_instr p (Zero) -> p.(prog) =
+           p'.(prog) -> p.(mem) = p'.(mem) ->
+           p'.(b) = p.(b) -> 0 = Common.to_nat p'.(ac) -> Common.to_nat p'.(pc) =
+           (Common.to_nat p.(pc)) + 1 ->
+           semantics p p'.
+End Assembly.
