first_attempt/Common.v
@@ -1,0 +1,73 @@
+Require Import Vector.
+Import Vector.VectorNotations.
+
+Require Import Coq.Program.Equality.
+Require Import Lia.
+
+Module Common.
+
+Definition embed {A : Type} {B : Type} (f : A -> B) :=
+   fun x y => y = f x.
+
+Inductive star {A : Type} (R : A -> A -> Prop) : A -> A -> Prop :=
+  | rt_refl : forall x, star R x x
+  | rt_trans : forall x y z, R x y -> star R y z -> star R x z.
+
+Theorem rt_step {A} (R : A -> A -> Prop) :
+  forall x y, R x y -> (star R) x y.
+Proof.
+  intros x y H.
+  apply rt_trans with (x := x) (y := y) (z := y).
+  assumption.
+  apply rt_refl.
+Qed.
+
+Inductive plus {A : Type} (R : A -> A -> Prop) : A -> A -> Prop :=
+  | t_base : forall x y, R x y -> plus R x y
+  | t_trans : forall x y z, R x y -> plus R y z -> plus R x z.
+
+Fixpoint to_nat {n} (x : Fin.t n) : nat :=
+  match x with
+  | Fin.F1 => 0
+  | Fin.FS t => 1 + (to_nat t)
+  end.
+
+Definition make_f1 (n : nat) (H : n <> 0) : Fin.t n.
+Proof.
+  destruct n eqn:H1.
+  - unfold not in H. assert (0 = 0). reflexivity. contradiction.
+  - exact Fin.F1.
+Defined.
+
+Definition make_fn (n : nat) (x : nat) (H : n <> 0) : Fin.t n :=
+  match Fin.of_nat x n with
+  | inleft p => p
+  | inright _ => make_f1 n H
+  end.
+
+Definition strengthen {n} (x : Fin.t (S n)) (H : Common.to_nat x <> n) : Fin.t n.
+Proof.
+  destruct n.
+  assert (x = Fin.F1).
+  dependent destruction x.
+  contradiction.
+  inversion x.
+  rewrite H0 in H.
+  contradiction.
+  apply Common.make_fn.
+  exact (Common.to_nat x).
+  lia.
+Defined.
+
+Definition minus {n} (x : Fin.t (S n)) (H : n <> 0) : Fin.t n.
+Proof.
+  destruct n eqn:H0.
+  - contradiction.
+  - destruct x eqn:H1.
+    + exact Fin.F1.
+    + apply Common.make_fn.
+      exact (Common.to_nat t).
+      unfold not. contradiction.
+Defined.
+
+End Common.
