first_attempt/Compiler.v
@@ -1,0 +1,257 @@
+Require Import Common.
+Require Import Language.
+Require Import Assembly.
+From Hammer Require Import Hammer.
+From Hammer Require Import Tactics.
+Require Import Vector.
+Import Vector.VectorNotations.
+Require Import Program.Equality.
+Require Import PeanoNat.
+Require Import Lia.
+Import Nat.
+Require Import Coq.Vectors.VectorEq.
+Require Coq.Program.Wf.
+
+Module Compiler.
+
+Definition lenvec {A n} (v : Vector.t A n) : nat := n.
+Fixpoint matched' {n} (p : Language.program n) (c : nat) : bool :=
+  match c with
+  | 0 => false
+  | _ => match p with
+    | [] => c =? 1
+    | Language.Jump :: l => matched' l (c+1)
+    | Language.Ret  :: l => matched' l (c-1)
+    | _ :: l => matched' l c
+    end
+  end.
+
+
+Inductive matched {n} (p : Language.program n) : Prop :=
+  | match_r : matched' p 1 = true -> matched p.
+Fixpoint comp_len {n} (p : Language.program n) : nat :=
+  match p with
+  | Vector.nil _ => 0
+  | Language.PtrInc :: xs => 1 + comp_len xs
+  | Language.PtrDec :: xs => 1 + comp_len xs
+  | Language.Inc :: xs => 6 + comp_len xs
+  | Language.Dec :: xs => 6 + comp_len xs
+  | Language.Jump :: xs => 2 + comp_len xs
+  | Language.Ret :: xs => 2 + comp_len xs
+  | Language.Halt :: xs => 1 + comp_len xs
+  end.
+
+Fixpoint compile'' {n} (p : Language.program n) :
+                          (Assembly.program (comp_len p)) :=
+  match p with
+  | [] => []
+  | Language.PtrInc :: h => (Assembly.Add 1) :: compile'' h
+  | Language.PtrDec :: h => (Assembly.Sub 1) :: compile'' h
+  | Language.Inc :: h =>  Assembly.Swap   ::
+                          Assembly.Load   ::
+                          Assembly.Add 1  ::
+                          Assembly.Store  ::
+                          Assembly.Zero   ::
+                          Assembly.Swap   :: compile'' h
+  | Language.Dec :: h =>  Assembly.Swap   ::
+                          Assembly.Load   ::
+                          Assembly.Sub 1  ::
+                          Assembly.Store  ::
+                          Assembly.Zero   ::
+                          Assembly.Swap   :: compile'' h
+
+  | Language.Jump :: h => Assembly.Skip   ::
+                          Assembly.UJUMP :: compile'' h
+  | Language.Ret :: h =>  Assembly.Skip   ::
+                          Assembly.URET :: compile'' h
+  | Language.Halt :: h => Assembly.Halt   :: compile'' h
+  end.
+
+Definition compile_first {n : nat} (i : Language.instr) : Assembly.instr :=
+  match i with
+  | Language.PtrInc => Assembly.Add 1
+  | Language.PtrDec => Assembly.Sub 1
+  | Language.Inc => Assembly.Swap
+  | Language.Dec => Assembly.Swap
+  | Language.Jump => Assembly.Skip
+  | Language.Ret => Assembly.Skip
+  | Language.Halt => Assembly.Halt
+  end.
+
+Fixpoint compile_index {n} (p : Language.program n) (x : Fin.t n) 
+                           : Fin.t (comp_len p).
+Proof.
+  destruct x eqn:H1; rewrite (eta p).
+  - destruct hd; apply Fin.F1.
+  - destruct hd.
+    + do 1 apply Fin.FS. apply compile_index. exact t0.
+    + do 1 apply Fin.FS. apply compile_index. exact t0.
+    + do 6 apply Fin.FS. apply compile_index. exact t0.
+    + do 6 apply Fin.FS. apply compile_index. exact t0.
+    + do 2 apply Fin.FS. apply compile_index. exact t0.
+    + do 2 apply Fin.FS. apply compile_index. exact t0.
+    + do 1 apply Fin.FS. apply compile_index. exact t0.
+Defined.
+
+Fixpoint nb_jump {n} (p : Assembly.program n) : nat :=
+  match p with
+  | [] => 0
+  | Assembly.UJUMP :: t => 1 + nb_jump t
+  | _ :: t => nb_jump t
+  end.
+
+Fixpoint nb_ret {n} (p : Assembly.program n) : nat :=
+  match p with
+  | [] => 0
+  | Assembly.URET :: t => 1 + nb_ret t
+  | _ :: t => nb_ret t
+  end.
+
+Fixpoint j_indexes {n} (p : Assembly.program n) 
+                       : (Vector.t (Fin.t n) (nb_jump p)) :=
+  match p with
+  | [] => []
+  | Assembly.UJUMP :: t => Fin.F1 :: map Fin.FS (j_indexes t)
+  | _ :: t => map Fin.FS (j_indexes t)
+  end.
+
+Fixpoint r_indexes {n} (p : Assembly.program n) 
+                       : (Vector.t (Fin.t n) (nb_ret p)) :=
+  match p with
+  | [] => []
+  | Assembly.URET :: t => Fin.F1 :: map Fin.FS (r_indexes t)
+  | _ :: t => map Fin.FS (r_indexes t)
+  end.
+
+  
+
+Fixpoint link_jump' {n ln ln'} (p : Assembly.program n) 
+                          (jumps : Vector.t (Fin.t n) ln)
+                          (rets : Vector.t (Fin.t n) ln') :
+                          Assembly.program n :=
+  match jumps with
+  | [] => p
+  | a :: jumps' => match rets with
+                  | [] => p
+                  | r :: rets' => link_jump' 
+                                  (replace p a (Assembly.Jump 
+                                  (Common.to_nat r)))
+                                  jumps' rets'
+                  end
+  end.
+
+
+Definition link_jump {n} (p : Assembly.program n) : (Assembly.program n) :=
+  link_jump' p (j_indexes p) (r_indexes p).
+
+Fixpoint nb_ljump {n} (p : Assembly.program n) : nat :=
+  match p with
+  | [] => 0
+  | Assembly.Jump _ :: t => 1 + nb_ljump t
+  | _ :: t => nb_ljump t
+  end.
+
+
+Fixpoint lj_indexes {n} (p : Assembly.program n) 
+                        : (Vector.t (Fin.t n) (nb_ljump p)) :=
+  match p with
+  | [] => []
+  | Assembly.Jump _ :: t => Fin.F1 :: map Fin.FS (lj_indexes t)
+  | _ :: t => map Fin.FS (lj_indexes t)
+  end.
+
+
+Definition make_f1 (x : nat) (H : x <> 0) : Fin.t x.
+Proof.
+  destruct x eqn:H1.
+  - auto with *.
+  - exact Fin.F1.
+Defined.
+
+Fixpoint weaken_fin_t {n : nat} (f : Fin.t n) : Fin.t (S n) :=
+  match f in Fin.t n return Fin.t (S n) with
+  | Fin.F1 => Fin.F1
+  | Fin.FS f' => Fin.FS (weaken_fin_t f')
+  end.
+
+Fixpoint make_indexes (n : nat) : Vector.t (Fin.t n) n :=
+  match n with
+  | 0 => []
+  | S i => Fin.F1 :: map Fin.FS (make_indexes i)
+  end.
+
+Fixpoint link_ret' {n ln ln'} (p : Assembly.program n) 
+                          (jumps : Vector.t (Fin.t n) ln) 
+                          (rets : Vector.t (Fin.t n) ln') :
+                          Assembly.program n :=
+  match rets with
+  | [] => p
+  | a :: rets' => match jumps with
+                  | [] => p
+                  | r :: jumps' => link_ret' (replace p a 
+                                   (Assembly.Jump (Common.to_nat r)))
+                                   jumps' rets'
+                  end
+  end.
+
+Definition inc_jump (i : Assembly.instr) : Assembly.instr :=
+  match i with
+  | Assembly.Jump n0 => Assembly.Jump (n0 + 1)
+  | a => a
+  end.
+
+Definition link_ret {n} (p : Assembly.program n) : (Assembly.program n) :=
+  (link_ret' p (lj_indexes p) (r_indexes p)).
+
+Definition link {n} (l : Assembly.program n) : (Assembly.program n) :=
+  map (inc_jump) (link_ret (link_jump l)).
+
+Definition make_vector (A : Type) (x : A) (n : nat) : Vector.t A n.
+Proof.
+  induction n.
+  - apply Vector.nil.
+  - apply Vector.cons.
+    + exact x.
+    + exact IHn.
+Defined.
+
+Lemma lm1 {n m} : forall p, n <> 0 -> comp_len (@Language.prog n m p) <> 0.
+Proof.
+  intros.
+  destruct p.
+  cbn.
+  destruct prog.
+  inversion pc.
+  unfold not. intros.
+  destruct h; inversion H0.
+Qed.
+
+Definition compile' {n m}
+  (p : Language.state (n := n)) (HA: n <> 0) (HA2 : m <> 0) : 
+  (Assembly.state (n := comp_len p.(Language.prog)) (m := m)) :=
+  let newlen := comp_len p.(Language.prog) in
+  let newpc := compile_index p.(Language.prog) p.(Language.pc) in
+  let f1_index := make_f1 (comp_len p.(Language.prog)) (lm1 p HA) in
+  let f1_mem := make_f1 m HA2 in
+  @Assembly.mkState newlen m (compile'' p.(Language.prog)) p.(Language.mem)
+   newpc p.(Language.ptr) f1_mem.
+
+Definition compile_link {n m} (p : Language.state (n := n)) (HA : n <> 0)
+                              (HA2 : m <> 0) : 
+  (Assembly.state (n := comp_len p.(Language.prog)) (m := m)) :=
+  let cpl := compile' p HA HA2 in
+  Assembly.mkState (comp_len (Language.prog p)) m (link cpl.(Assembly.prog))
+                   cpl.(Assembly.mem)
+  cpl.(Assembly.pc) cpl.(Assembly.ac) cpl.(Assembly.b).
+
+Inductive compile {n m}
+  (p : Language.state (n := n))
+  (q : Assembly.state (n := comp_len p.(Language.prog)) (m := m)) : Prop :=
+  | comp_r : forall H H1, matched (p.(Language.prog)) -> q 
+             = compile_link p H H1 -> compile p q.
+End Compiler.
+
+Require Import ExtrOcamlBasic.
+Require Import ExtrOcamlNatInt.
+Extraction Language OCaml.
+Recursive Extraction Compiler.compile_link.
