first_attempt/Language.v
@@ -1,0 +1,111 @@
+Require Import Vector.
+Import Vector.VectorNotations.
+Require Import Program.Equality.
+Require Import PeanoNat.
+Require Import Common.
+Require Import Lia.
+Module Language.
+Inductive instr : Type :=
+  | PtrInc : instr
+  | PtrDec : instr
+  | Inc : instr
+  | Dec : instr
+  | Jump : instr
+  | Ret : instr
+  | Halt : instr.
+Definition program (n : nat) := t instr n.
+
+Record state {n m : nat} : Type := mkState
+{ 
+  prog : program n;
+  mem : t nat m;
+  pc : Fin.t n;
+  ptr : Fin.t m;
+}.
+
+Definition read_instr' {n} (prog : program n) (pc : Fin.t n) : instr :=
+ prog[@pc].
+
+Inductive read_instr {n m} (p : state) (i : instr) : Prop  :=
+  | ri : read_instr' p.(prog n m) p.(pc n m) = i -> read_instr p i.
+
+Definition read_mem' {m} (mem : t nat m) (ptr : Fin.t m) : nat := mem[@ptr].
+
+Inductive read_mem {n m} (p : state) (e : nat) : Prop  :=
+  | mi : read_mem' p.(mem n m) p.(ptr n m) = e -> read_mem p e.
+
+
+Inductive mem_diff {m} (m1 : t nat m) (m2 : t nat m) (x : Fin.t m) : Prop :=
+  | md : (forall i, i <> x -> m2[@i] = m1[@i]) -> mem_diff m1 m2 x. 
+
+
+Definition option_inc (i : option nat) : option nat :=
+  match i with
+  | None => None
+  | Some a => Some (a + 1)
+  end.
+
+Fixpoint matching_ret' {n} (l : t instr n) (idx : nat) (c c' : nat) :
+                           option nat :=
+  match l with
+  | [] => None
+  | i :: h => if c' <=? idx then matching_ret' h idx c (c'+1) else
+    match i with
+    | Jump => matching_ret' h idx (c+1) (c'+1)
+    | Ret => if c =? 0 then (Some (c' + 1)) else matching_ret' h idx
+             (c-1) (c'+1)
+    | _ => matching_ret' h idx c (c'+1)
+  end
+end.
+
+Fixpoint matching_jump' {n} (l : t instr n) (idx : nat) (c : nat) 
+                        (c' : option nat) : option nat :=
+  match l with
+  | [] => None
+  | Jump :: h => if c =? idx then None else matching_jump' h idx (c+1) (Some c)
+  | Ret :: h => if c =? idx then (option_inc c') else None
+  | _ :: h => if c =? idx then None else matching_jump' h idx (c+1) c'
+  end.
+
+Inductive matching_jump {n} (p : program n) (x : Fin.t n) (x' : Fin.t n) : Prop :=
+  | mj : matching_jump' p (Common.to_nat x) 0 None = Some (Common.to_nat x') -> matching_jump p x x'.
+Inductive matching_ret {n} (p : program n) (x : Fin.t n) (x' : Fin.t n): Prop :=
+  | mr : matching_ret' p (Common.to_nat x) 0 0 = Some (Common.to_nat x') -> matching_ret p x x'.
+
+(*Some cases will not be accepted for compilation anyway, like unmatched jumps.*)
+(* Small-step operational semantics for our source language.*)
+
+Inductive semantics {n m} (p : state) (p' : state) : Prop :=
+  | ptr_inc : read_instr p PtrInc ->  Common.to_nat p.(ptr) + 1 = Common.to_nat p'.(ptr) ->
+                   Common.to_nat p.(pc n m) + 1 = Common.to_nat p'.(pc)-> p.(prog) = p'.(prog) ->
+                   p.(mem) = p'.(mem) -> semantics p p'
+  | ptr_dec : read_instr p PtrDec -> Common.to_nat p.(ptr) - 1 = Common.to_nat p'.(ptr) ->
+                    Common.to_nat p.(pc) +1 = Common.to_nat p'.(pc)-> p.(prog) = p'.(prog) ->
+                   p.(mem) = p'.(mem) -> semantics p p'
+  | inc : read_instr p Inc -> p.(ptr) = p'.(ptr) ->
+               Common.to_nat p.(pc) +1 = Common.to_nat p'.(pc)-> p.(prog) = p'.(prog) ->
+               mem_diff p.(mem) p'.(mem) p.(ptr) ->
+               p.(mem)[@p.(ptr)] + 1 = p'.(mem)[@p.(ptr)] ->
+               semantics p p'
+  | dec : read_instr p Dec -> p.(ptr) = p'.(ptr) ->
+               Common.to_nat p.(pc) +1 = Common.to_nat p'.(pc)-> p.(prog) = p'.(prog) ->
+               mem_diff p.(mem) p'.(mem) p.(ptr) ->
+               p.(mem)[@p.(ptr)] - 1 = p'.(mem)[@p.(ptr)] ->
+               semantics p p'
+  | jump_z : read_instr p Jump -> p.(ptr) = p'.(ptr) ->
+                  p.(prog) = p'.(prog) -> p.(mem) = p'.(mem) ->
+                  read_mem p 0 -> matching_ret p.(prog) p.(pc) p'.(pc) ->
+                  semantics p p'
+  | jump_nz : read_instr p Jump -> p.(ptr) = p'.(ptr) ->
+                   p.(prog) = p'.(prog) -> p.(mem) = p'.(mem) ->
+                   ~ (read_mem p 0) ->
+                   Common.to_nat p.(pc) + 1 = Common.to_nat p'.(pc)-> semantics p p'
+  | ret_z :  read_instr p Ret -> p.(ptr) = p'.(ptr) ->
+                  p.(prog) = p'.(prog) -> p.(mem) = p'.(mem) ->
+                  matching_jump p.(prog) p.(pc) p'.(pc) -> read_mem p 0 ->
+                  semantics p p'
+  | ret_nz : read_instr p Ret -> p.(ptr) = p'.(ptr) ->
+                  p.(prog) = p'.(prog) -> p.(mem) = p'.(mem) ->
+                  ~ (read_mem p 0) ->
+                  Common.to_nat p.(pc) +  1 = Common.to_nat p'.(pc) -> semantics p p'.
+End Language.
