first_attempt/Simulation.v
@@ -1,0 +1,144 @@
+Require Import Common. 
+Module Simulation.
+
+Definition lockstep_forward_sim {A : Type} {B : Type} 
+  (compile : A -> B -> Prop)
+  (eval : A -> A -> Prop)
+  (eval': B -> B -> Prop) := 
+    forall p q, compile p q ->
+    forall p', eval p p' -> 
+    exists q', compile p' q' /\ eval' q q'.
+
+Definition lockstep_backward_sim {A : Type} {B : Type} 
+  (compile : A -> B -> Prop)
+  (eval : A -> A -> Prop)
+  (eval': B -> B -> Prop) := 
+    forall p q, compile p q ->
+    forall q', eval' q q' -> 
+    exists p', compile p' q' /\ eval p p'.
+
+Definition lockstep_bisim {A : Type} {B : Type} 
+  (compile : A -> B -> Prop)
+  (eval : A -> A -> Prop)
+  (eval': B -> B -> Prop) := 
+    forall p q, compile p q ->
+    (forall p', eval p p' -> 
+    exists q', eval' q q' /\ compile p' q') /\
+    (forall q', eval' q q' -> 
+    exists p', eval p p' /\ compile p' q').
+
+Definition plus_forward_sim {A : Type} {B : Type}
+  (compile : A -> B -> Prop)
+  (eval : A -> A -> Prop)
+  (eval': B -> B -> Prop) :=
+    forall p q, compile p q ->
+    forall p', eval p p' ->
+    exists q', compile p' q' /\ (Common.plus eval') q q'.
+
+Definition plus_backward_sim {A : Type} {B : Type}
+  (compile : A -> B -> Prop)
+  (eval : A -> A -> Prop)
+  (eval': B -> B -> Prop) :=
+    forall p q, compile p q ->
+    forall q', eval' q q' ->
+    exists p', (Common.plus eval) p p' /\ compile p' q'.
+
+Definition plus_bisim {A : Type} {B : Type} 
+  (compile : A -> B -> Prop)
+  (eval : A -> A -> Prop)
+  (eval': B -> B -> Prop) := 
+    forall p q, compile p q ->
+    (forall p', eval p p' -> 
+    exists q', (Common.plus eval') q q' /\ compile p' q') /\
+    (forall q', eval' q q' -> 
+    exists p', (Common.plus eval) p p' /\ compile p' q').
+
+Definition star_forward_sim {A : Type} {B : Type} {Ord : Type}
+  (measure : A -> Ord)
+  (order_R : Ord -> Ord -> Prop) 
+  (compile : A -> B -> Prop)
+  (eval : A -> A -> Prop)
+  (eval': B -> B -> Prop) :=
+    forall p q, compile p q ->
+    (forall p', eval p p' ->
+    exists q', (Common.plus eval') q q' /\ compile p' q') \/
+    (forall p', eval p p' /\ order_R (measure p') (measure p) ->
+    exists q', (Common.star eval') q q' /\ compile p' q').
+
+Definition star_backward_sim {A : Type} {B : Type} {Ord : Type}
+  (measure : B -> Ord)
+  (order_R : Ord -> Ord -> Prop) 
+  (compile : A -> B -> Prop)
+  (eval : A -> A -> Prop)
+  (eval': B -> B -> Prop) :=
+    forall p q, compile p q ->
+    (forall q', eval' q q' ->
+    exists p', (Common.plus eval) p p' /\ compile p' q') \/
+    (forall q', eval' q q' /\ order_R (measure q') (measure q) ->
+    exists p', (Common.star eval) p p' /\ compile p' q').
+
+Definition star_bisim {A : Type} {B : Type} {Ord : Type} {Ord' : Type}
+  (measure : A -> Ord)
+  (measure' : B -> Ord')
+  (order_R : Ord -> Ord -> Prop)
+  (order_R' : Ord' -> Ord' -> Prop)
+  (compile : A -> B -> Prop)
+  (eval : A -> A -> Prop)
+  (eval': B -> B -> Prop) :=
+    forall p q, compile p q ->
+    ((forall p', eval p p' ->
+    exists q', (Common.plus eval') q q' /\ compile p' q') \/
+    (forall p', eval p p' /\ order_R (measure p') (measure p) ->
+    exists q', (Common.star eval') q q' /\ compile p' q')) /\
+    ((forall q', eval' q q' ->
+    exists p', (Common.plus eval) p p' /\ compile p' q') \/
+    (forall q', eval' q q' /\ order_R' (measure' q') (measure' q) ->
+    exists p', (Common.star eval) p p' /\ compile p' q')).
+
+Definition option_forward_sim {A : Type} {B : Type} {Ord : Type}
+  (empty : (A -> A -> Prop) -> (A -> A -> Prop))
+  (measure : A -> Ord)
+  (order_R : Ord -> Ord -> Prop) 
+  (compile : A -> B -> Prop)
+  (eval : A -> A -> Prop)
+  (eval': B -> B -> Prop) :=
+    forall p q, compile p q ->
+    (forall p', eval p p' ->
+    exists q', eval' q q' /\ compile p' q') \/
+    (forall p', (empty eval) p p' /\ order_R (measure p') (measure p) ->
+    compile p' q).
+
+Definition option_backward_sim {A : Type} {B : Type} {Ord : Type}
+  (empty : (B -> B -> Prop) -> (B -> B -> Prop))
+  (measure : B -> Ord)
+  (order_R : Ord -> Ord -> Prop) 
+  (compile : A -> B -> Prop)
+  (eval : A -> A -> Prop)
+  (eval': B -> B -> Prop) :=
+    forall p q, compile p q ->
+    (forall q', eval' q q' ->
+    exists p', eval p p' /\ compile p' q') \/
+    (forall q', (empty eval') q q' /\ order_R (measure q') (measure q) ->
+    compile p q').
+
+Definition option_bisim {A : Type} {B : Type} {Ord : Type} {Ord' : Type}
+  (empty : (A -> A -> Prop) -> (A -> A -> Prop))
+  (empty': (B -> B -> Prop) -> (B -> B -> Prop))
+  (measure : A -> Ord)
+  (measure' : B -> Ord')
+  (order_R : Ord -> Ord -> Prop)
+  (order_R' : Ord' -> Ord' -> Prop)
+  (compile : A -> B -> Prop)
+  (eval : A -> A -> Prop)
+  (eval': B -> B -> Prop) :=
+    forall p q, compile p q ->
+    ((forall p', eval p p' ->
+    exists q', eval' q q' /\ compile p' q') \/
+    (forall p', (empty eval) p p' /\ order_R (measure p') (measure p) ->
+    compile p' q)) /\
+    ((forall q', eval' q q' ->
+    exists p', eval p p' /\ compile p' q') \/
+    (forall q', (empty' eval') q q' /\ order_R' (measure' q') (measure' q) ->
+    compile p q')).
+
+End Simulation.
