first_attempt/Verification.v
@@ -1,0 +1,446 @@
+Require Import Common.
+Require Import Language.
+Require Import Assembly.
+Require Import Simulation.
+Require Import Compiler.
+Require Import Lia.
+Require Import Vector.
+Import Vector.VectorNotations.
+Require Import Program.Equality.
+Require Import PeanoNat.
+
+From Hammer Require Import Hammer.
+From Hammer Require Import Tactics.
+
+Import Nat.
+Module Verification.
+
+Definition eval {n m} := @Language.semantics n m.
+Definition eval' {n m} := @Assembly.semantics n m.
+
+Lemma comp_len_eq : forall n m p p', eval p p' ->
+                    @Compiler.comp_len n (@Language.prog n m p) =
+                    @Compiler.comp_len n (@Language.prog n m p').
+Proof.
+  intros.
+  assert (p.(Language.prog) = p'.(Language.prog)).
+  + inversion H; assumption.
+  + inversion H0.
+    reflexivity.
+Defined.
+
+Definition comp_len_f
+ {n n' m p p'} (H : eval p p') 
+ (q : @Assembly.state (@Compiler.comp_len n (@Language.prog n m p')) n') 
+ : @Assembly.state (@Compiler.comp_len n (@Language.prog n m p)) n'.
+Proof.
+  assert (@Compiler.comp_len n (@Language.prog n m p) =
+          @Compiler.comp_len n (@Language.prog n m p')).
+  - apply comp_len_eq.
+    assumption.
+  - rewrite H0.
+    exact q.
+Defined.
+  
+Lemma match_tr {n m} : forall p p', Compiler.matched (n := n) (Language.prog p) ->
+                       eval p p' -> Compiler.matched (Language.prog p' (m := m)).
+Proof.
+  intros.
+  assert (Language.prog p = Language.prog p').
+  - inversion H0; assumption.
+  - rewrite <- H1.
+    assumption.
+Qed.
+
+Lemma comp_link_prog {n m} : forall p HA HA1 q, Compiler.compile_link p HA HA1 = q ->
+                             q.(Assembly.prog) =
+                             Compiler.link (@Compiler.compile'' n p.(@Language.prog n m)).
+Proof.
+  intros.
+  rewrite <- H.
+  assert (Assembly.prog
+  {|
+    Assembly.prog := Compiler.link (Assembly.prog (Compiler.compile' p HA HA1));
+    Assembly.mem := Assembly.mem (Compiler.compile' p HA HA1);
+    Assembly.pc := Assembly.pc (Compiler.compile' p HA HA1);
+    Assembly.ac := Assembly.ac (Compiler.compile' p HA HA1);
+    Assembly.b := Assembly.b (Compiler.compile' p HA HA1)
+  |} = Compiler.link (Assembly.prog (Compiler.compile' p HA HA1))).
+  now reflexivity.
+  unfold Compiler.compile_link.
+  rewrite H0.
+  f_equal.
+Qed.
+
+Definition len_asm (i : Assembly.instr) : nat :=
+  match i with
+  | Assembly.Add 1 => 1
+  | Assembly.Sub 1 => 1
+  | Assembly.Swap => 6
+  | Assembly.Skip => 2
+  | Assembly.Halt => 1
+  | _ => 0
+  end.
+
+Definition vec_len {A n} (v : Vector.t A n) : nat := n.
+
+Lemma read_instr_eq {n} : forall p i,
+                          (Compiler.compile'' p)[@@Compiler.compile_index n p i]
+                          = @Compiler.compile_first n p[@i].
+Proof.
+  induction i; dependent destruction p;
+  destruct h; simpl;
+  try (now reflexivity);
+  try (apply IHi).
+Qed.
+
+Lemma link_stable : forall n p ind i, (i <> Assembly.UJUMP /\ i <> Assembly.URET) ->
+                    p[@ind] = i -> (@Compiler.link n p)[@ind] = i.
+Proof.
+Admitted.
+
+Lemma read_comp {n m} : forall p i H1 H2, Language.read_instr p i ->
+                               i <> Language.Jump -> i <> Language.Ret ->
+                               Assembly.read_instr (@Compiler.compile_link n m p H1 H2)
+                               (@Compiler.compile_first n i).
+Proof.
+  unfold Compiler.compile_link.
+  unfold Compiler.compile'.
+  intros.
+  ssimpl.
+  apply Assembly.ri.
+  unfold Assembly.read_instr'. simpl.
+  assert ((Compiler.compile'' prog)[@Compiler.compile_index prog pc] =
+  @Compiler.compile_first n prog[@pc]).
+  apply read_instr_eq.
+  apply link_stable.
+  ssimpl.
+  - unfold Compiler.compile_first in H4.
+    qsimpl.
+  - unfold Compiler.compile_first in H4.
+    qsimpl.
+  - qsimpl.
+Qed.
+
+Lemma to_nat_st {n} : forall a b, @Common.to_nat n a = Common.to_nat b -> a = b.
+Proof.
+  intros.
+  dependent induction a; dependent destruction b.
+  reflexivity.
+  assert (n = 0). ssimpl. exfalso. ssimpl.
+  assert (n = 0). ssimpl. exfalso. ssimpl.
+  f_equal.
+  apply IHa.
+  inversion H.
+  reflexivity.
+Qed.
+
+Fixpoint weaken_fin_t {n : nat} (f : Fin.t n) : Fin.t (S n) :=
+  match f in Fin.t n return Fin.t (S n) with
+  | Fin.F1 => Fin.F1
+  | Fin.FS f' => Fin.FS (weaken_fin_t f')
+  end.
+
+Definition safe_fs {n} (i : Fin.t n) (H : (Common.to_nat i) + 1 <> n) : Fin.t n.
+Proof.
+  intros.
+  destruct n. inversion i.
+  pose (X := Fin.of_nat (Common.to_nat i + 1) (S n)).
+  destruct X eqn:A.
+  exact t0.
+  sfirstorder.
+Defined.
+
+Lemma fs_lm : forall n i, @Common.to_nat n i <> n.
+Proof.
+  intros.
+  induction i, n.
+  - simpl. lia.
+  - simpl. lia.
+  - inversion i.
+  - sfirstorder.
+Qed.
+
+Lemma safe_fs_is_s {n} : forall i H,
+                         @Common.to_nat n (safe_fs i H) = (Common.to_nat i) + 1.
+Proof.
+  intros.
+  induction i, n.
+  - simpl in H. lia.
+  - now reflexivity.
+  - inversion i.
+  - hauto.
+Qed.
+
+Lemma not_final_lm1 {n} : forall prog pc pc',
+                          (@Common.to_nat n pc) + 1 = @Common.to_nat n pc' ->
+                          Common.to_nat (Compiler.compile_index prog pc) + 1 <>
+                          Compiler.comp_len prog.
+Proof.
+  intros;
+  assert (Common.to_nat pc' <> n) by apply fs_lm;
+  rewrite <- H in H0;
+  induction pc; dependent destruction pc'; dependent destruction prog.
+  - sfirstorder.
+  - simpl; dependent destruction pc'; dependent destruction prog; qsimpl.
+  - simpl in H; inversion H.
+  - ssimpl; (apply IHpc with (prog := prog) (pc' := pc'); (try assumption);
+    try hauto).
+Qed.
+ 
+Lemma not_final {n} : forall pc prog spc,
+                     (Common.to_nat pc) + 1 = @Common.to_nat n spc ->
+                     exists sqpc, @Common.to_nat (Compiler.comp_len prog) sqpc =
+                     (Common.to_nat (@Compiler.compile_index n prog pc) + 1).
+Proof.
+  intros.
+  assert (Common.to_nat (@Compiler.compile_index n prog pc) + 1 
+          <> Compiler.comp_len prog).
+  apply not_final_lm1 with (pc' := spc); assumption.
+  exists (safe_fs (@Compiler.compile_index n prog pc) H0); 
+  apply safe_fs_is_s.
+Qed.
+
+Lemma compiled_pc : forall n prog pc pc0 i, Language.read_instr' prog pc0 = i ->
+                    Common.to_nat pc0 + 1 = Common.to_nat pc ->
+                    Common.to_nat (Compiler.compile_index prog pc0) +
+                    vec_len (Compiler.compile'' [i])
+                    = Common.to_nat (@Compiler.compile_index n prog pc).
+Proof.
+  intros.
+  unfold vec_len.
+  unfold Language.read_instr' in *.
+  induction pc0; dependent destruction pc; dependent destruction prog.
+  - sfirstorder.
+  - ssimpl; dependent destruction pc; dependent destruction prog; ssimpl.
+  - simpl in H. destruct i; destruct h; ssimpl.
+  - simpl in H. destruct h; destruct i; hauto; do 6 f_equal; assumption. 
+Qed.
+
+Theorem seq_instr {n} : forall p x x'
+                  (off : Fin.t (Compiler.comp_len ([p[@x]]))),
+                  Common.to_nat x' =
+                  Common.to_nat (@Compiler.compile_index n p x) + Common.to_nat off ->
+                  (Compiler.compile'' p)[@x'] = (Compiler.compile'' [p[@x]])[@off].
+Proof.
+Admitted.
+
+Ltac seq_ins_n p pc' n H :=
+  intros;
+  destruct p as [prog mem pc ptr];
+  unfold Compiler.compile_link in *;
+  apply Assembly.ri;
+  unfold Assembly.read_instr' in *;
+  simpl in *;
+  destruct H; try ssimpl;
+  apply link_stable; try sdone;
+  assert (Compiler.comp_len [prog[@pc]] <> 0) as EH2;
+  try qauto;
+  pose (X := Common.make_fn (Compiler.comp_len [prog[@pc]]) n EH2);
+  assert ((Compiler.compile'' prog)[@pc'] = (Compiler.compile'' [prog[@pc]])[@X]) as EH;
+  try (apply seq_instr); hauto.
+
+Lemma seq_inc1 {n m}: forall p q1 H H',
+                     (Language.prog p)[@Language.pc p] = Language.Inc ->
+                     Assembly.read_instr (Compiler.compile_link p H H') Assembly.Swap ->
+                     eval' (@Compiler.compile_link n m p H H') q1 ->
+                     Assembly.read_instr q1 Assembly.Load.
+Proof.
+  seq_ins_n p pc0 1 H2.
+Qed.
+
+Lemma seq_inc2 {n m}: forall p q1 q2 H H',
+                     (Language.prog p)[@Language.pc p] = Language.Inc ->
+                     Assembly.read_instr (Compiler.compile_link p H H') Assembly.Swap ->
+                     eval' (@Compiler.compile_link n m p H H') q1 ->
+                     eval' q1 q2 -> Assembly.read_instr q1 Assembly.Load ->
+                     Assembly.read_instr q2 (Assembly.Add 1).
+Proof.
+  seq_ins_n p pc0 2 H3.
+Qed.
+
+Lemma seq_inc3 {n m}: forall p q1 q2 q3 H H',
+                     (Language.prog p)[@Language.pc p] = Language.Inc ->
+                     Assembly.read_instr (Compiler.compile_link p H H') Assembly.Swap ->
+                     eval' (@Compiler.compile_link n m p H H') q1 ->
+                     eval' q1 q2 -> eval' q2 q3 -> Assembly.read_instr q1 Assembly.Load ->
+                     Assembly.read_instr q2 (Assembly.Add 1) ->
+                     Assembly.read_instr q3 (Assembly.Store).
+Proof.
+  seq_ins_n p pc0 3 H4.
+Qed.
+Lemma seq_inc4 {n m}: forall p q1 q2 q3 q4 H H',
+                     (Language.prog p)[@Language.pc p] = Language.Inc ->
+                     Assembly.read_instr (Compiler.compile_link p H H') Assembly.Swap ->
+                     eval' (@Compiler.compile_link n m p H H') q1 ->
+                     eval' q1 q2 -> eval' q2 q3 -> eval' q3 q4 ->
+                     Assembly.read_instr q1 Assembly.Load ->
+                     Assembly.read_instr q2 (Assembly.Add 1) ->
+                     Assembly.read_instr q3 (Assembly.Store) ->
+                     Assembly.read_instr q4 (Assembly.Zero).
+Proof.
+  (*seq_ins_n p pc0 4 H5.*) (*works, but too slow*)
+Admitted.
+Lemma seq_inc5 {n m}: forall p q1 q2 q3 q4 q5 H H',
+                     (Language.prog p)[@Language.pc p] = Language.Inc ->
+                     Assembly.read_instr (Compiler.compile_link p H H') Assembly.Swap ->
+                     eval' (@Compiler.compile_link n m p H H') q1 ->
+                     eval' q1 q2 -> eval' q2 q3 -> eval' q3 q4 -> eval' q4 q5 ->
+                     Assembly.read_instr q1 Assembly.Load ->
+                     Assembly.read_instr q2 (Assembly.Add 1) ->
+                     Assembly.read_instr q3 (Assembly.Store) ->
+                     Assembly.read_instr q4 (Assembly.Zero) ->
+                     Assembly.read_instr q5 (Assembly.Swap).
+Proof.
+  (*seq_ins_n p pc0 5 H6.*) (*too slow*)
+Admitted.
+
+Theorem comp_correct {n m : nat} :
+    forall p q, Compiler.compile p q -> 
+    forall p' (E : eval p p'), 
+    exists q', Compiler.compile p' q' /\
+    (Common.plus eval') q (comp_len_f (n := n) (n' := m) E q').
+Proof.
+  intros.
+  assert (n <> 0).
+  inversion H. assumption.
+  assert (m <> 0).
+  inversion H. assumption.
+  exists (Compiler.compile_link p' H0 H1).
+  split.
+  - apply Compiler.comp_r with (H := H0) (H1 := H1).
+    + assert (Compiler.matched (Language.prog p)).
+      inversion H.
+      assumption.
+      apply match_tr with (p := p); assumption.
+    + reflexivity. 
+  - (unfold comp_len_f; unfold eq_rec_r; unfold eq_rec; unfold eq_rect).
+    ssimpl.
+    (*Assembly.PtrInc*)
+    + apply Common.t_base.
+      apply Assembly.add with (n' := 1).
+      * assert (Assembly.read_instr (@Compiler.compile_link n m {|Language.prog := prog;
+       Language.mem := mem;
+       Language.pc := pc0;
+       Language.ptr := ptr0|} H2 H3) (Assembly.Add 1)).
+       apply read_comp with (i := Language.PtrInc). ssimpl.
+       discriminate. discriminate.
+       assumption.
+      * simpl.
+        unfold Common.to_nat.
+        apply compiled_pc with (i := Language.PtrInc); assumption.
+      * now reflexivity.
+      * now reflexivity.
+      * simpl. unfold Compiler.make_f1. ssimpl.
+      * ssimpl.
+    (*Assembly.PtrDec*)
+    + apply Common.t_base.
+      apply Assembly.sub with (n' := 1).
+      * assert (Assembly.read_instr (@Compiler.compile_link n m {|Language.prog := prog;
+       Language.mem := mem;
+       Language.pc := pc0;
+       Language.ptr := ptr0|} H2 H3) (Assembly.Sub 1)).
+       apply read_comp with (i := Language.PtrDec). ssimpl.
+       discriminate. discriminate.
+       assumption.
+      * simpl.
+        apply compiled_pc with (i := Language.PtrDec); assumption.
+      * now reflexivity.
+      * now reflexivity.
+      * simpl. unfold Compiler.make_f1. ssimpl.
+      * ssimpl.
+
+    (*Assembly.Inc*)
+    + remember (Compiler.compile_link {|Language.prog := prog;Language.mem := mem0;
+               Language.pc := pc0; Language.ptr := ptr|} H2 H3) as q.
+      remember (Compiler.compile_link {|Language.prog := prog;Language.mem := mem;
+               Language.pc := pc; Language.ptr := ptr|} H0 H1) as q'.
+      assert (prog[@pc0] = Language.Inc). ssimpl.
+      assert (Compiler.compile'' [Language.Inc] =
+             [Assembly.Swap; Assembly.Load; Assembly.Add 1;
+             Assembly.Store;Assembly.Zero; Assembly.Swap]).
+      now reflexivity.
+
+      assert (Assembly.read_instr 
+             (@Compiler.compile_link n m {|Language.prog := prog;
+                                           Language.mem := mem0;
+                                           Language.pc := pc0;
+                                           Language.ptr := ptr|} H2 H3)
+                                           (Assembly.Swap)).
+      apply read_comp with (i := Language.Inc).
+      ssimpl.
+      discriminate. discriminate.
+(**)
+      assert (exists q1, eval' q q1).
+      rewrite <- Heqq in *.
+      assert (exists sqpc,
+              @Common.to_nat (Compiler.comp_len prog) sqpc =
+              (Common.to_nat (Assembly.pc q) + 1)).
+      ssimpl.
+      apply not_final with (spc := pc).
+      assumption.
+      destruct H7; rename x into sqpc.
+      exists (Assembly.mkState _ _  (Assembly.prog q) (Assembly.mem q)
+                                    (sqpc) (Assembly.b q)
+                                    (Assembly.ac q)).
+      ssimpl.
+      destruct H7; rename x into q1.
+
+      assert (Assembly.read_instr q1 Assembly.Load).
+      apply seq_inc1 with (H := H2) (H' := H3); ssimpl.
+      assert (exists q2, eval' q1 q2).
+      admit.
+      destruct H9; rename x into q2.
+      assert (Assembly.read_instr q2 (Assembly.Add 1)).
+      admit.
+      assert (exists q3, eval' q2 q3).
+      admit.
+      destruct H11; rename x into q3.
+      assert (Assembly.read_instr q3 Assembly.Store).
+      admit.
+      assert (exists q4, eval' q3 q4).
+      admit.
+      destruct H13; rename x into q4.
+      assert (Assembly.read_instr q4 Assembly.Zero).
+      admit.
+      assert (exists q5, eval' q4 q5).
+      admit.
+      destruct H15; rename x into q5.
+      assert (Assembly.read_instr q5 Assembly.Swap).
+      admit.
+      apply Common.t_trans with (y := q1). assumption.
+      apply Common.t_trans with (y := q2). assumption.
+      apply Common.t_trans with (y := q3). assumption.
+      apply Common.t_trans with (y := q4). assumption.
+      apply Common.t_trans with (y := q5). assumption.
+      apply Common.t_base.
+      apply Assembly.swap.
+      * assumption.
+      * assert (Assembly.prog q = Assembly.prog q').
+        ssimpl.
+        assert (Assembly.prog q1 = Assembly.prog q). inversion H7; qsimpl.
+        assert (Assembly.prog q2 = Assembly.prog q1). inversion H9; qsimpl.
+        assert (Assembly.prog q3 = Assembly.prog q2). inversion H11; qsimpl.
+        assert (Assembly.prog q4 = Assembly.prog q3). inversion H13; qsimpl.
+        assert (Assembly.prog q5 = Assembly.prog q4). inversion H15; qsimpl.
+        qsimpl.
+      * admit.
+      * admit.
+      * admit.
+      * admit.
+
+    + (*same proof as before*) 
+      (*Assembly.Dec*) 
+      admit.
+    + (*Assembly.Jump, resulting from two cases of Jump and two cases of Ret*)
+      (* will require other lemmas, as we will have to consider linking: *)
+      (*assert the existence of q1*)
+      admit.
+    + (*assert the existence of q1*)
+      admit.
+    + (*assert the existence of q1*) 
+      admit.
+    + (*assert the existence of q1*)
+      admit.
+Admitted.
+End Verification.
