first_attempt/prototype/Example.v
@@ -1,0 +1,107 @@
+Require Import Vector.
+Import Vector.VectorNotations.
+Require Import Program.Equality.
+
+Inductive instr1 : Type :=
+  | Load : instr1
+  | Halt : instr1.
+
+Inductive instr2 {n} : Type :=
+  | Load' : instr2
+  | Halt' : Fin.t n -> instr2.
+
+Definition make_f1 (x : nat) (H : x <> 0) : Fin.t x.
+Proof.
+  destruct x eqn:H1.
+  - auto with *.
+  - exact Fin.F1.
+Defined.
+
+Definition comp_instr {n : nat} (HA : n <> 0) x :=
+  match x with
+  | Load => Load'
+  | Halt => Halt' (make_f1 n HA)
+  end.
+
+Fixpoint comp_len {n} (p : t instr1 n) : nat :=
+  match p with
+  | Vector.nil _ => 0
+  | Halt :: xs => 1 + comp_len xs
+  | Load :: xs => 2 + comp_len xs
+  end.
+
+Fixpoint compile' {n n'} (HA : n' <> 0) (p : t instr1 n) : t (@instr2 n') (comp_len p).
+Proof.
+  destruct p.
+  - exact [].
+  - destruct h.
+    + cbn.
+      exact ((Load' :: Load' :: (compile' n n' HA p))).
+    + cbn.
+      exact ((Halt' (make_f1 n' HA)) :: (compile' n n' HA p)).
+Defined.
+
+Fixpoint to_nat {n} (x : Fin.t n) : nat.
+Proof.
+  destruct x eqn:H.
+  - exact 0.
+  - apply plus.
+    + exact 1.
+    + apply to_nat with (n := n).
+      exact t.
+Defined.
+
+Fixpoint weaken_fin_t {n : nat} (f : Fin.t n) : Fin.t (S n) :=
+  match f in Fin.t n return Fin.t (S n) with
+  | Fin.F1 => Fin.F1
+  | Fin.FS f' => Fin.FS (weaken_fin_t f')
+  end.
+Require Import Coq.Program.Wf.
+From Hammer Require Import Tactics.
+Require Import Lia.
+Program Fixpoint fin_t_fact {n} (i : Fin.t n) {measure (to_nat i)} : nat :=
+  match i with
+  | Fin.F1 => 1
+  | Fin.FS t => (to_nat i) * (fin_t_fact (weaken_fin_t t))
+  end.
+Next Obligation.
+  dependent destruction t.
+  - ssimpl.
+  - ssimpl.
+    assert (to_nat (weaken_fin_t t) = to_nat t).
+    + dependent induction t. ssimpl.
+      ssimpl.
+    + rewrite H. lia.
+Qed.
+Check (nat, bool).
+
+Fixpoint make_indexes (n : nat) : Vector.t (Fin.t n) n :=
+  match n with
+  | 0 => []
+  | S i => Fin.F1 :: map Fin.FS (make_indexes i)
+  end.
+
+Compute (make_indexes 8).
+
+Lemma lm1 : forall n p, n <> 0 -> @comp_len n p <> 0.
+Proof.
+  intros. destruct p. auto with *. destruct h; cbn; auto with *.
+Qed.
+Definition compile {n : nat} (p : t instr1 n) (HA : n <> 0) : t (@instr2 (comp_len p)) (comp_len p) :=
+  @compile' n (comp_len p) (lm1 n p HA) p.
+
+Fixpoint compile_index {n} (p : t instr1 n) (x : Fin.t n) : Fin.t (comp_len p).
+Proof.
+  destruct x eqn:H1; rewrite (eta p); destruct hd eqn:H2.
+  - apply Fin.F1.
+  - apply Fin.F1.
+  - do 2 apply Fin.FS. apply compile_index. exact t.
+  - do 1 apply Fin.FS, compile_index. exact t.
+Defined.
+
+Theorem th : forall {n} (x : Fin.t n) (p : Vector.t instr1 n) (HA : n <> 0),
+  @comp_instr (comp_len p) (lm1 n p HA) p[@x] = (@compile n p HA)[@compile_index p x].
+Admitted.
+
+
+
